split off 'Node' from the rest of the cyclic buffer so it can be allocated on its own NUMA node

concurrency/node-replication/Impl.i.dfy
@@ -14,6 +14,10 @@ module Impl(nrifc: NRIfc) {
   import opened RwLockImpl
   import opened Runtime
 
+  /*
+   * Anything which is allocated on a NUMA node
+   */
+
   linear datatype NodeReplica = NodeReplica(
     linear actual_replica: nrifc.DataStructureType,
     glinear ghost_replica: Replica
@@ -26,53 +30,60 @@ module Impl(nrifc: NRIfc) {
   }
 
   linear datatype Node = Node(
-    linear localTail: Atomic<uint64, LocalTail>,
-    linear replica: RwLock<NodeReplica>
+    linear replica: RwLock<NodeReplica>,
+    nodeId: uint64
+  )
+  {
+    predicate WF() {
+      && (forall nodeReplica :: replica.inv(nodeReplica) <==> nodeReplica.WF(nodeId as int))
+    }
+  }
+
+  /*
+   * Central cyclic buffer stuff
+   */
+
+  linear datatype NodeInfo = NodeInfo(
+    linear localTail: Atomic<uint64, LocalTail>
   )
   {
     predicate WF(nodeId: NodeId) {
-      && (forall v, g :: atomic_inv(localTail, v, g) <==>
-          g == LocalTail(nodeId, v as int))
-      && (forall nodeReplica :: replica.inv(nodeReplica) <==>
-          nodeReplica.WF(nodeId)) 
+      && (forall v, g :: atomic_inv(localTail, v, g) <==> g == LocalTail(nodeId, v as int))
     }
   }
   
   linear datatype NR = NR(
     linear ctail: Atomic<uint64, Ctail>,
-    linear nodes: lseq<Node>
+    linear node_info: lseq<NodeInfo>
   )
   {
     predicate WF() {
-      && (forall v, g :: atomic_inv(ctail, v, g) <==>
-          g == Ctail(v as int))
-      && (forall nodeId | 0 <= nodeId < |nodes| ::
-          nodes[nodeId].WF(nodeId))
+      && (forall v, g :: atomic_inv(ctail, v, g) <==> g == Ctail(v as int))
+      && (forall nodeId | 0 <= nodeId < |node_info| :: node_info[nodeId].WF(nodeId))
     }
   }
 
-  method do_read(shared nr: NR, op: nrifc.ReadonlyOp, glinear ticket: Readonly)
+  method do_read(shared nr: NR, shared node: Node, op: nrifc.ReadonlyOp,
+      glinear ticket: Readonly)
   returns (result: nrifc.ReturnType, glinear stub: Readonly)
   requires nr.WF()
+  requires node.WF()
   // The contract for this method works like this:
   // Input a ticket which "allows" us to perform the readonly operation specified
   // by the input parameter `op`
   requires ticket.rs == ReadonlyInit(op)
   // And we must return a stub that validates that we performed the operation
   // with the result being that value that we are returning.
-  ensures stub == Readonly(ticket.rid, ReadonlyDone(result))
+  ensures stub.rid == ticket.rid && stub.rs.ReadonlyDone? && stub.rs.ret == result
   decreases * // method is not guaranteed to terminate
   {
-    // TODO get nodeId value from somewhere
-    var nodeId := Runtime.CurrentNumaNode();
-
     // 1. Read ctail
     atomic_block var ctail := execute_atomic_load(nr.ctail) {
       ghost_acquire ctail_token; // declares ctail_token as a 'glinear' object
       assert ctail_token == Ctail(ctail as int); // this follows from the invariant on nr.ctail
 
       // perform transition of ghost state here ...
-      var stub := perform_TransitionReadonlyReadCtail(ticket, ctail_token);
+      stub := perform_TransitionReadonlyReadCtail(ticket, ctail_token);
 
       ghost_release ctail_token;
     }
