concurrency/node-replication/Runtime.s.dfy
@@ -1,7 +1,7 @@
 // Copyright 2018-2021 VMware, Inc., Microsoft Inc., Carnegie Mellon University, ETH Zurich, and University of Washington
 // SPDX-License-Identifier: BSD-2-Clause
 
-module {:extern "LinearExtern"} Runtime {
+module {:extern "Runtime"} Runtime {
   method {:extern "LinearExtern", "CurrentNumaNode"} CurrentNumaNode()
     returns (node: nat) // Well this probably should be u64 but don't know what to include
     ensures node < 4 as nat // Who needs more than 4 numa nodes?
